Cleanup the tutorial a bit

tests/lean/Tutorial.lean
@@ -6,32 +6,35 @@ open Result
 
 namespace Tutorial
 
-/- # Simple Arithmetic Example ################################################# -/
+/-#===========================================================================#
+  #
+  #     Simple Arithmetic Example
+  #
+  #===========================================================================#-/
 
-/- As a first step, we want to consider the function below which performs
-   simple arithmetic. There are several things to note.
+/- As a first example, let's consider the function below.
  -/
 
 def mul2_add1 (x : U32) : Result U32 := do
   let x1 ← x + x
-  let x2 ← x1 + (U32.ofInt 1)
+  let x2 ← x1 + 1#u32
   ret x2
 
-/- # Machine integers
+/- There are several things to note.
+
+   # Machine integers
+   ==================
    Because Rust programs manipulate machine integers which occupy a fixed
-   size in memory, we model integers with types like [U32], which are simply
-   bounded integers. [U32.ofInt 1] is simply the machine integer constant 1.
+   size in memory, we model integers by using types like [U32], which is
+   the type of integers which take their values between 0 and 2^32 - 1 (inclusive).
+   [1#u32] is simply the constant 1 (seen as a [U32]).
 
-   Because machine integers are bounded, arithmetic operations can fail, for instance
-   because of an overflow: this is the reason why the output of [mul2_add1] uses
-   the [Result] type.
-
-   You can see a definition or its type by using the #print and #check commands.
+   You can see a definition or its type by using the [#print] and [#check] commands.
    It is also possible to jump to definitions (right-click + "Go to Definition"
    in VS Code).
 
    For instance, you can see below that [U32] is defined in terms of a more generic
-   type [Scalar] (just move the cursor to the #print command below).
+   type [Scalar] (just move the cursor to the [#print] command below).
 
  -/
 #print U32 -- This shows the definition of [U32]
@@ -40,24 +43,29 @@ def mul2_add1 (x : U32) : Result U32 := do
 #print mul2_add1 -- This show the full definition of [mul2_add1]
 
 /- # Syntax
+   ========
+   Because machine integers are bounded, arithmetic operations can fail, for instance
+   because of an overflow: this is the reason why the output of [mul2_add1] uses
+   the [Result] type. In particular, addition can fail.
+
    We use a lightweight "do"-notation to write code which calls potentially failing
    functions. In practice, all our function bodies start with a [do] keyword,
-   which indicates to Lean we want to use this lightweight syntax, and after
-   the do, instead of writing let-bindings as [let x1 := ...], we write them
-   as: [let x1 ← ...]. We also have lightweight notations for common operations
-   like the addition.
-
-   *Remark:* in order to type the left-arrow [←] you can type: [\l]. Generally
-   speaking, your editor can tell you how to type the symbols you see in .lean
-   files. For instance in VS Code, you can simply hover your mouse over the
-   symbol and a pop-up window will open displaying all the information you need.
+   which enables using this lightweight syntax. After the [do], instead of writing
+   let-bindings as [let x1 := ...], we write them as: [let x1 ← ...]. We also
+   have lightweight notations for common operations like the addition.
 
    For instance, in [let x1 ← x + x], the [x + x] expression desugars to
    [Scalar.add x x] and the [let x1 ← ...] desugars to a call to [bind].
 
    The definition of [bind x f] is worth investigating. It simply checks whether
-   [x : Result ...] successfully evaluated to some result, in which case it
-   calls [f] with this result, propagating the error otherwise.
+   [x : Result ...] successfully evaluates to some value, in which case it
+   calls [f] with this value, and propagates the error otherwise. See the output
+   of the [#print] command below.
+
+   *Remark:* in order to type the left-arrow symbol [←] you can type: [\l]. Generally
+   speaking, your editor can tell you how to type the symbols you see in Lean
+   code. For instance in VS Code, you can simply hover your mouse over the
+   symbol and a pop-up window will open displaying all the information you need.
  -/
 #print Primitives.bind
 
@@ -91,17 +99,14 @@ theorem mul2_add1_spec
   /- The precondition (we give it the name "h" to be able to refer to it in the proof).
      We simply state that [2 * x + 1] must not overflow.
 
-     The ↑ notation (\u) is used to coerce values. Here, we coerce [x], which is
-     a bounded machine integer, to an unbounded mathematical integer. Note that
-     writing [↑ x] is the same as writing [x.val].
-
-     Remark: we advise always writing inequalities in the same direction (that is
-     ≤ and not ≥), because it helps the simplifier.
+     The ↑ notation ("\u") is used to coerce values. Here, we coerce [x], which is
+     a bounded machine integer, to an unbounded mathematical integer, which is
+     easier to work with. Note that writing [↑x] is the same as writing [x.val].
    -/
-  (h : 2 * (↑ x) + 1 ≤ U32.max)
+  (h : 2 * ↑x + 1 ≤ U32.max)
   /- The postcondition -/
   : ∃ y, mul2_add1 x = ret y ∧  -- The call succeeds
-  ↑ y = 2 * (↑ x) + (1 : Int)   -- The output has the expected value
+  ↑ y = 2 * ↑x + (1 : Int)   -- The output has the expected value
   := by
   /- The proof -/
   -- Start by a call to the rewriting tactic to reveal the body of [mul2_add1]
@@ -111,25 +116,27 @@ theorem mul2_add1_spec
      Doing this properly requires a few manipulations: we need to instantiate
      the theorem, introduce it in the context, destruct it to introduce [x1], etc.
      We automate this with the [progress] tactic: [progress with th as ⟨ x1 .. ⟩]
-     uses theorem [th], rename the output to [x1] and further decomposes the
-     postcondition of [th] (it is possible to provide more inputs to name the
-     assumptions introduced by the postcondition, for instance: [as ⟨ x1, h ⟩]).
+     uses theorem [th], instantiates it properly by looking at the goal, renames
+     the output to [x1] and further decomposes the postcondition of [th].
 
-     If you look at the goal after the call to [progress], you wil see there is
-     a new variable [x1] and an assumption stating that [↑ x1 = ↑ x + ↑ x].
+     Note that it is possible to provide more inputs to name the assumptions
+     introduced by the postcondition (for instance: [as ⟨ x1, h ⟩]).
 
-     Also, [U32.add_spec] has the precondition that the addition doesn't overflow.
+     If you look at the goal after the call to [progress], you wil see that:
+     - there is a new variable [x1] and an assumption stating that [↑x1 = ↑x + ↑x]
+     - the call [x + x] disappeared from the goal: we "progressed" by one step
+
+     Remark: the theorem [U32.add_spec] actually has a precondition, namely that
+     the addition doesn't overflow.
      In the present case, [progress] manages to prove this automatically by using
      the fact that [2 * x + 1 < U32.max]. In case [progress] fails to prove a
      precondition, it leaves it as a subgoal.
    -/
-  progress with U32.add_spec as ⟨ x1 .. ⟩
+  progress with U32.add_spec as ⟨ x1 ⟩
   /- We can call [progress] a second time for the second addition -/
-  progress with U32.add_spec as ⟨ x2 .. ⟩
+  progress with U32.add_spec as ⟨ x2 ⟩
   /- We are now left with the remaining goal. We do this by calling the simplifier
-     then [scalar_tac], a tactic to solve linear arithmetic problems (i.e.,
-     arithmetic problems in which there are not multiplications between two
-     variables): 
+     then [scalar_tac], a tactic to solve arithmetic problems:
    -/
   simp at *
   scalar_tac
@@ -141,13 +148,14 @@ theorem mul2_add1_spec
    For this reason, we provide the possibility of registering theorems in a database
    so that [progress] can automatically look them up. This is done by marking
    theorems with custom attributes, like [pspec] below.
+
    Theorems in the standard library like [U32.add_spec] have already been marked with such
    attributes, meaning we don't need to tell [progress] to use them.
  -/
 @[pspec] -- the [pspec] attribute saves the theorem in a database, for [progress] to use it
-theorem mul2_add1_spec2 (x : U32) (h : 2 * (↑ x) + 1 ≤ U32.max)
+theorem mul2_add1_spec2 (x : U32) (h : 2 * ↑x + 1 ≤ U32.max)
   : ∃ y, mul2_add1 x = ret y ∧
-  ↑ y = 2 * (↑ x) + (1 : Int)
+  ↑ y = 2 * ↑x + (1 : Int)
   := by
   rw [mul2_add1]
   progress as ⟨ x1 .. ⟩ -- [progress] automatically lookups [U32.add_spec]
@@ -163,16 +171,21 @@ def use_mul2_add1 (x : U32) (y : U32) : Result U32 := do
   x1 + y
 
 @[pspec]
-theorem use_mul2_add1_spec (x : U32) (y : U32) (h : 2 * (↑ x) + 1 + ↑ y ≤ U32.max) :
+theorem use_mul2_add1_spec (x : U32) (y : U32) (h : 2 * ↑x + 1 + ↑y ≤ U32.max) :
   ∃ z, use_mul2_add1 x y = ret z ∧
-  ↑ z = 2 * (↑ x) + (1 : Int) + ↑ y := by
+  ↑z = 2 * ↑x + (1 : Int) + ↑y := by
   rw [use_mul2_add1]
   -- Here we use [progress] on [mul2_add1]
   progress as ⟨ x1 .. ⟩
   progress as ⟨ z .. ⟩
   simp at *; scalar_tac
 
-/- # Recursion ################################################################ -/
+
+/-#===========================================================================#
+  #
+  #     Recursion
+  #
+  #===========================================================================#-/
 
 /- We can have a look at more complex examples, for example recursive functions. -/
 
@@ -216,17 +229,17 @@ open CList
 divergent def list_nth (T : Type) (l : CList T) (i : U32) : Result T :=
   match l with
   | CCons x tl =>
-    if i = U32.ofInt 0
-    then Result.ret x
+    if i = 0#u32
+    then ret x
     else do
-           let i1 ← i - (U32.ofInt 1)
-           list_nth T tl i1
-  | CNil => Result.fail Error.panic
+      let i1 ← i - 1#u32
+      list_nth T tl i1
+  | CNil => fail Error.panic
 
 /- Conversion to Lean's standard list type.
 
-   Note that because we define the function as belonging to the namespace
-   [CList], we can use the notation [l.to_list] if [l] has type [CList ...].
+   Note that because we use the suffix "CList.", we can use the notation [l.to_list]
+   if [l] has type [CList ...].
  -/
 def CList.to_list {α : Type} (x : CList α) : List α :=
   match x with
@@ -235,45 +248,52 @@ def CList.to_list {α : Type} (x : CList α) : List α :=
 
 /- Let's prove that [list_nth] indeed accesses the ith element of the list.
 
-   About the parameter [Inhabited T]: this tells us that we must have an instance of the
+   Remark: the parameter [Inhabited T] tells us that we must have an instance of the
    typeclass [Inhabited] for the type [T].  As of today we can only use [index] with
    inhabited types, that is to say types which are not empty (i.e., for which it is
    possible to construct a value - for instance, [Int] is inhabited because we can exhibit
    the value [0: Int]). This is a technical detail.
+
+   Remark: we didn't mention it before, but we advise always writing inequalities
+   in the same direction (that is: use [<] and not [>]), because it helps the simplifier.
+   More specifically, if you have the assumption that [x > y] in the context, the simplifier
+   may not be able to rewrite [y < x] to [⊤].
  -/
 theorem list_nth_spec {T : Type} [Inhabited T] (l : CList T) (i : U32)
   -- Precondition: the index is in bounds
-  (h : (↑ i) < l.to_list.len)
+  (h : ↑i < l.to_list.len)
   -- Postcondition
   : ∃ x, list_nth T l i = ret x ∧
-  x = l.to_list.index (↑ i)
+  -- [x] is the ith element of [l] after conversion to [List]
+  x = l.to_list.index ↑i
   := by
-  -- Here we can to be careful when unfolding the body of [list_nth]: we could
+  -- Here we have to be careful when unfolding the body of [list_nth]: we could
   -- use the [simp] tactic, but it will sometimes loop on recursive definitions.
   rw [list_nth]
-  -- Let's simply follow the structure of the function
+  -- Let's simply follow the structure of the function, by first matching on [l]
   match l with
   | CNil =>
-    -- We can't get there: we can derive a contradiction from the precondition
+    -- We can't get there: we can derive a contradiction from the precondition:
+    -- we have that [i < 0] (because [i < CNil.to_list.len]) and at the same
+    -- time [0 ≤ i] (because [i] is a [U32] unsigned integer).
     -- First, let's simplify [to_list CNil] to [0]
     simp [CList.to_list] at h
-    -- Proving we have a contrdiction: this is just linear arithmetic (note that
-    -- [U32] integers are unsigned, that is, they are greater than or equal to 0).
+    -- Proving we have a contradiction
     scalar_tac
   | CCons hd tl =>
-    -- Simplifying the match
+    -- Simplify the match
     simp only []
-    -- Cases on i
+    -- Perform a case disjunction on [i].
     -- The notation [hi : ...] allows us to introduce an assumption in the
-    -- context, to use the fact that in the branches we have [i = U32.ofInt 0]
-    -- and [¬ i = U32.ofInt 0]
-    if hi: i = U32.ofInt 0 then
-      -- We can finish the proof simply by using the simplier.
+    -- context, to remember the fact that in the branches we have [i = 0#u32]
+    -- and [¬ i = 0#u32].
+    if hi: i = 0#u32 then
+      -- We can finish the proof simply by using the simplifier.
       -- We decompose the proof into several calls on purpose, so that it is
       -- easier to understand what is going on.
       -- Simplify the condition and the [if then else]
       simp [hi]
-      -- Proving the final equality
+      -- Prove the final equality
       simp [CList.to_list]
     else
       -- The interesting branch
@@ -282,7 +302,7 @@ theorem list_nth_spec {T : Type} [Inhabited T] (l : CList T) (i : U32)
       -- i0 := i - 1
       progress as ⟨ i1, hi1 ⟩
       -- [progress] can handle recursion
-      simp [CList.to_list] at h
+      simp [CList.to_list] at h -- we need to simplify this inequality to prove the precondition
       progress as ⟨ l1 ⟩
       -- Proving the postcondition
       -- We need this to trigger the simplification of [index to.to_list i.val]
@@ -294,10 +314,14 @@ theorem list_nth_spec {T : Type} [Inhabited T] (l : CList T) (i : U32)
       -- by giving it [*] as argument, we tell [simp] to use all the assumptions
       -- to perform rewritings. In particular, it will use [i.val ≠ 0] to
       -- apply [List.index_nzero_cons].
-      have : i.val ≠ 0 := by scalar_tac
+      have : i.val ≠ 0 := by scalar_tac -- Remark: [simp at hi] also works
       simp [CList.to_list, *]
 
-/- # Partial functions  ################################################# -/
+/-#===========================================================================#
+  #
+  #     Partial Functions
+  #
+  #===========================================================================#-/
 
 /- Recursive functions may not terminate on all inputs.
 
@@ -310,28 +334,31 @@ theorem list_nth_spec {T : Type} [Inhabited T] (l : CList T) (i : U32)
    We will skip the details of how [divergent] precisely handles non-termination.
    All you need to know is that the [Result] type has actually 3 cases (we saw
    the first 2 cases in the examples above):
-   - ret: successful computation
-   - fail: failure (panic because of overflow, etc.)
-   - div: the computation doesn't terminate.
+   - [ret]: successful computation
+   - [fail]: failure (panic because of overflow, etc.)
+   - [div]: the computation doesn't terminate
 
    If in a theorem we state and prove that:
    ```
    ∃ y, i32_id x = ret x
    ```
    we not only prove that the function doesn't fail, but also that it terminates.
+
+   *Remark*: in practice, whenever Aeneas generates a recursive function, it
+   annotates it with the [divergent] keyword.
  -/
 divergent def i32_id (x : I32) : Result I32 :=
-  if x = I32.ofInt 0 then ret (I32.ofInt 0)
+  if x = 0#i32 then ret 0#i32
   else do
-    let x1 ← x - I32.ofInt 1
+    let x1 ← x - 1#i32
     let x2 ← i32_id x1
-    x2 + (I32.ofInt 1)
+    x2 + 1#i32
 
 /- We can easily prove that [i32_id] behaves like the identity on positive inputs -/
 theorem i32_id_spec (x : I32) (h : 0 ≤ x.val) :
   ∃ y, i32_id x = ret y ∧ x.val = y.val := by
   rw [i32_id]
-  if hx : x = I32.ofInt 0 then
+  if hx : x = 0#i32 then
     simp_all
   else
     simp [hx]
@@ -344,6 +371,9 @@ theorem i32_id_spec (x : I32) (h : 0 ≤ x.val) :
     -- Postcondition
     simp; scalar_tac
 -- Below: we have to prove that the recursive call performed in the proof terminates.
+-- Otherwise, we could prove any result we want by simply writing a theorem which
+-- uses itself in the proof.
+--
 -- We first specify a decreasing value. Here, we state that [x], seen as a natural number,
 -- decreases at every recursive call.
 termination_by i32_id_spec x _ => x.val.toNat
